\documentclass[main]{subfiles}

\begin{document}

\begin{remark}
It is easy to see that $\underline\Hom(\mathbbm1,Y)\cong Y$ since $\Hom(-,Y)\cong\Hom(-,\underline\Hom(\mathbbm1, Y))$ is the representable functor
\end{remark}

\begin{remark}[Definition of $^tf:Y^\vee\to X^\vee$]
\[\Hom(Y^\vee,X^\vee)\cong\Hom(Y^\vee\otimes X,\mathbbm 1)\cong\Hom(X,\underline{\Hom}(Y^\vee,\mathbbm1))\cong\Hom(X,Y^{\vee\vee})\]
And there is a canonical choice of $X\to X^{\vee\vee}$ given by $\operatorname{ev}$ in $\Hom(X^\vee\otimes X,\mathbbm1)\cong\Hom(X,X^{\vee\vee})$
\end{remark}


\end{document}