\documentclass[main]{subfiles}

\begin{document}

\begin{proposition}
\begin{align*}
\int_0^\infty\frac{x^{s-1}}{e^x-1}dx&=\int_0^\infty x^{s-1}e^{-x}\sum_{n=0}^\infty e^{-nx}dx \\
&=\sum_{n=1}^\infty\int_0^\infty x^{s-1}e^{-nx}dx \\
&=\sum_{n=1}^\infty\frac{1}{n^s}\int_0^\infty x^{s-1}e^{-x}dx \\
&=\sum_{n=1}^\infty\frac{1}{n^s}\Gamma(s) \\
&=\zeta(s)\Gamma(s)
\end{align*}
\end{proposition}

\begin{theorem}[Euler's reflection formula]
$\Gamma(z)\Gamma(1-z)=\dfrac{\pi}{\sin(\pi z)}$, $z\notin\mathbb Z$
\end{theorem}

\end{document}