\documentclass[main]{subfiles}

\begin{document}

\begin{definition}
Chen's \textit{iterated integral} is defined to be
\[\int_\gamma\omega_1(t)\cdots\omega_n(t)=\int\displaylimits_{0\leq t_1\leq\cdots\leq t_n\leq 1}\gamma^*\omega_1(t_1)\wedge\cdots\wedge\gamma^*\omega_n(t_n)\]
\end{definition}

\begin{theorem}\cite{Zhao_MultipleZetaFunctionsMultiplePolylogarithmsAndTheirSpecialValues}
\begin{enumerate}[leftmargin=*]
\item Inversion
\[\int_\gamma\omega_1(t)\cdots\omega_n(t)=(-1)^n\int_\gamma\omega_n(t)\cdots\omega_1(t)\]
\item Path composition ($\gamma_1(1)=\gamma_2(0)$)
\[\int_{\gamma_2\circ\gamma_1}\omega_1(t)\cdots\omega_n(t)=\sum_{i=0}^n\int_{\gamma_1}\omega_1(t)\cdots\omega_i(t)\int_{\gamma_2}\omega_{i+1}(t)\cdots\omega_n(t)\]
\item Shuffle Product
\[\int_{\gamma}\omega_1(t)\cdots\omega_m(t)\int_{\gamma}\omega_{m+1}(t)\cdots\omega_{m+n}(t)=\sum_{\sigma\text{ runs over all $(m,n)$ shuffles}}\int_{\gamma}\omega_{\sigma^{-1}(1)}(t)\cdots\omega_{\sigma^{-1}(1)}(t)\]
\item Homotopy invariance \\
$\displaystyle\int_\gamma\sum_{j=1}^n\omega_1^{(j)}\cdots\omega_m^{(j)}$ is homotopy invariant if $\omega_i^{(j)}$ are closed and $\displaystyle\sum_j\omega_{i-1}^{(j)}\wedge\omega_i^{(j)}=0$
\end{enumerate}
\end{theorem}

under the standard choice of path
\[I(0;a_1,\cdots,a_n;1)=\int_{0<t_1<\cdots<t_n<1}\frac{dt_1}{t_1-a_1}\wedge\cdots\wedge\frac{dt_n}{t_n-a_n}\]

\begin{theorem}[Differential of iterated integrals]
\[dI(a_0;a_1,\cdots,a_n;a_{n+1})=\sum_{i=1}^nI(a_0;a_1,\cdots,\widehat{a_i},\cdots,a_n;a_{n+1})d\log\frac{(a_{i+1}-a_i)}{a_{i+1}-a_i}\]
\end{theorem}

\begin{proof}
$dI(a_0;a_1,\cdots,a_n;a_{n+1})$ is
\begin{equation*}
\scalemath{0.8}{
\begin{split}
&\sum_{i=1}^n\int_{a_0<t_1<\cdots<t_n<a_{n+1}}\frac{dt_1}{t_1-a_1}\wedge\cdots\wedge\frac{dt_i}{(t_i-a_i)^2}\wedge\cdots\wedge\frac{dt_n}{t_n-a_n}da_i\\
&=\sum_{i=1}^{n}\int_{a_0<t_1<\cdots<t_{i-1}<t_{i+1}<\cdots<t_n<a_{n+1}}\frac{dt_1}{t_1-a_1}\wedge\cdots\wedge\left(\frac{1}{t_{i-1}-a_{i}}-\frac{1}{t_{i+1}-a_{i}}\right)\wedge\cdots\wedge\frac{dt_n}{t_n-a_n}da_i\\
&=\sum_{i=1}^n\int_{a_0<t_1<\cdots<t_{i-1}<t_{i+1}<\cdots<t_n<a_{n+1}}\frac{dt_1}{t_1-a_1}\wedge\cdots\wedge\frac{dt_{i-1}}{(t_{i-1}-a_{i-1})(t_{i-1}-a_{i})}\wedge\cdots\wedge\frac{dt_n}{t_n-a_n}da_i \\
&-\sum_{i=1}^n\int_{a_0<t_1<\cdots<t_{i-1}<t_{i+1}<\cdots<t_n<a_{n+1}}\frac{dt_1}{t_1-a_1}\wedge\cdots\wedge\frac{dt_{i+1}}{(t_{i+1}-a_{i})(t_{i+1}-a_{i+1})}\wedge\cdots\wedge\frac{dt_n}{t_n-a_n}da_i\\
&=
\end{split}
}
\end{equation*}

$dI(0;a_1,\cdots,a_n;1)$ with respect to $a_i$ is \[\int_{0<t_1<\cdots<t_n<1}\frac{dt_1}{t_1-a_1}\wedge\cdots\wedge\frac{dt_i}{(t_i-a_i)^2}\wedge\cdots\wedge\frac{dt_n}{t_n-a_n}\]
By Fubini, we can first do integration
\[\int_{t_{i-1}}^{t_{i+1}}\frac{dt_i}{(t_i-a_i)^2}=\frac{1}{t_{i-1}-a_{i}}-\frac{1}{t_{i+1}-a_{i}}\]
On the other hand
\end{proof}

\end{document}