\documentclass[main]{subfiles}

\begin{document}

The following identity is true
\[\Li_{1,1}(x,y)=\Li_2\left(\frac{xy-y}{1-y}\right)-\Li_2\left(\frac{y}{y-1}\right)-\Li_2(xy)\]
\[\Li_2(1-x)=-\Li2(x)-\log x\log(1-x)+\frac{\pi^2}{6}\]
Note that $\log x\log(1-x)\to0$ as $x\to 1$

\begin{align*}
\Li_{1,1}(x,y)&=\int \frac{dy}{1-y}\frac{dx}{1-x}+\frac{d(xy)}{1-xy}\left(\frac{dy}{1-y}-\frac{dx}{x(1-x)}\right) \\
&=\int d\log(1-y)d\log(1-x)+d\log(1-xy)d\log\frac{x(1-y)}{1-x} \\
&=\int dv_2dv_1+dv_{12}dw_1
\end{align*}
To compute the monodromy around $x=0$, take $q(\epsilon)$ to be the loop $(x=\epsilon e^{it},y=\epsilon)$, we get $0$. \\
To compute the monodromy around $y=0$, take $q(\epsilon)$ to be the loop $(x=\epsilon,y=\epsilon e^{it})$, we get $0$. \\
To compute the monodromy around $x=1$, take $q(\epsilon)$ to be the composition of $(x=(1-t)\epsilon+t(1-\epsilon),y=\epsilon)$, $(x=1-\epsilon e^{it},y=\epsilon)$ and $(x=(1-t)(1-\epsilon)+t\epsilon,y=\epsilon)$, we get $0$. \\
To compute the monodromy around $y=1$, take $q(\epsilon)$ to be the composition of $(x=\epsilon,y=(1-t)\epsilon+t(1-\epsilon))$, $(x=\epsilon,y=1-\epsilon e^{it})$ and $(x=\epsilon,y=(1-t)(1-\epsilon)+t\epsilon)$, we get $-2\pi i\Li_1(x)$. \\
To compute the monodromy around $xy=1$, take $q$ to be the loop $(x=x^0,y\text{ such that }\int_qd\log(1-xy)=2\pi i)$, we get $-2\pi i\Li_1(\frac{1-xy}{1-x})$

The variation matrix is
\[\Lambda=\begin{bmatrix}
1&&&\\
\Li_1(y)&1&&\\
\Li_1(xy)&&1&\\
\Li_{1,1}(x,y)&\Li_1(x)&\Li_1\left(\frac{1-xy}{1-x}\right)&1
\end{bmatrix}\tau_{1,1}(2\pi i)\]
\[\omega=\begin{bmatrix}
0&&&\\
-dv_2&0&&\\
-dv_{12}&0&0&\\
0&-dv_1&-dw_1&0
\end{bmatrix}\]
Note that $\Li_1\left(\frac{1-xy}{1-x}\right)=-\log\left(\frac{x(y-1)}{1-x}\right)=\Li_1(y)-\Li_1(x^{-1})=\Li_1(y)-\Li_1(x)-\log x-i\pi$ \\
The monodromy representation $\rho$ is as follows \\
For monodromy around $x=0$
\[\begin{bmatrix}
1&&& \\
&1&& \\
&&1& \\
&&-1&1
\end{bmatrix}\]
For monodromy around $y=0$, identity. \\
For monodromy around $x=1$
\[\begin{bmatrix}
1&&& \\
&1&& \\
&&1& \\
&-1&1&1
\end{bmatrix}\]
For monodromy around $y=1$
\[\begin{bmatrix}
1&&& \\
-1&1&& \\
&&1& \\
&&-1&1
\end{bmatrix}\]
For monodromy around $xy=1$
\[\begin{bmatrix}
1&&& \\
&1&& \\
-1&&1& \\
&&&1
\end{bmatrix}\]

$\widehat{\mathcal L}_{1,1}(x)=\Li_{1, 1}(x,y) - \frac{1}{2}v_{12} v_2 - \frac{1}{2}v_1 v_2 + \frac{1}{2}v_1 v_{12} - \frac{1}{2}u_1 v_{12}$

\end{document}