\documentclass[main]{subfiles}

\begin{document}

\[\left[\begin{smallmatrix}
1\\
\Li_{1}(z)&1\\
\Li_{1}(yz)&0&1\\
\Li_{1}(xyz)&0&0&1\\
\Li_{1,1}(y,z)&\Li_1(y)&\Li_1(\frac{1-yz}{1-y})&0&1\\
\Li_{1,1}(xy,z)&\Li_1(xy)&0&\Li_1(\frac{1-xyz}{1-xy})&0&1\\
\Li_{1,1}(x,yz)&0&\Li_1(x)&\Li_1(\frac{1-xyz}{1-x})&0&0&1\\
\Li_{2}(xyz)&0&0&\log(xyz)&0&0&0&1\\
\Li_{1,1,1}(x,y,z)&\Li_{1,1}(x,y)&\Li_1(x)\Li_1(\frac{1-yz}{1-y})&\Li_{1,1}(\frac{1-xy}{1-x},\frac{1-xyz}{1-xy})&\Li_1(x)&\Li_1(\frac{1-xy}{1-x})&\Li_1(\frac{1-yz}{1-y})&0&1\\
\Li_{2,1}(xy,z)&\Li_2(xy)&0&\Li_2(x^{-1}y^{-1})-\Li_2(z)+\Li_1(z)\log(xyz)&0&\log(xy)&0&\Li_1(z)&0&1\\
\Li_{2,1}(x,yz)&0&\Li_2(x)&\Li_2(x^{-1})-\Li_2(yz)+\Li_1(yz)\log(xyz)&0&0&\log x&\Li_1(yz)&0&0&1\\
\Li_{2,1,1}(x,y,z)&\Li_{2,1}(x,y)&\Li_2(x)\Li_1(\frac{1-yz}{1-y})&\Li_{1,1,1}(\frac{1-y^{-1}z^{-1}}{1-z^{-1}},\frac{1}{1-y^{-1}z^{-1}},1-x^{-1}y^{-1}z^{-1})&\Li_2(x)&-\Li_{1,1}(1-x,\frac{1-xy}{1-x})&\log x\Li_1(\frac{1-yz}{1-y})&\Li_{1,1}(y,z)&\log x &\Li_1(y)&\Li_1(\frac{1-yz}{1-y})&1
\end{smallmatrix}\right]\]
\begin{align*}
\int_{(xyz)^{-1}}^1\frac{dt}{(yz)^{-1}-t}\frac{dt}{z^{-1}-t}&=\Li_{1,1}(y,z)+(u_1-v_1-\pi i)(u_{12}-v_{12}-\pi i)-\int_0^1\frac{dt}{x-t}\frac{dt}{xy-t}
\end{align*}
\[\omega=\left[\begin{smallmatrix}
0\\
-dv_3&0\\
-dv_{23}&0&0\\
-dv_{123}&0&0&0\\
&-dv_2&-w_{2,3}&0&0\\
&-dv_{12}&0&-dw_{12,3}&0&0\\
&&-dv_1&-dw_{1,23}&0&0&0\\
&&&du_{123}&0&0&0&0\\
&&&&-dv_1&-dw_{1,2}&-dw_{2,3}&0&0\\
&&&&&du_{12}&0&-dv_3&0&0\\
&&&&&&du_1&-dv_{23}&0&0&0\\
&&&&&&&&du_1&-dv_2&dw_{2,3}&0
\end{smallmatrix}\right]\]
Monodromy around $x=0,1$, $y=0,1$, $xy=1$, $z=0$ are $0$ \\
Monodromy around $z=1$ is $-2\pi i\Li_{2,1}(x,y)$ \\
Monodromy around $yz=1$ is $-2\pi i\Li_2(x)\Li_{1,1}(\frac{1-yz}{1-y})$ \\
Monodromy around $xyz=1$ is $-2\pi iI((xyz)^{-1};0,(yz)^{-1},z^{-1};1)$ \\
The monodromy representation $\rho$ is as follows \\
For monodromy around $x=0$
\[\begin{bmatrix}
1\\
&1\\
&&1\\
&&&1\\
&&&&1\\
&&&-1&&1\\
&&&-1&&&1\\
&&&1&&&&1\\
&&&&&-1&&&1\\
&&&&&1&&&&1\\
&&&&&&1&&&&1\\
&&&&&&&&1&&&1
\end{bmatrix}\]
For monodromy around $y=0$
\[\begin{bmatrix}
1\\
&1\\
&&1\\
&&&1\\
&&-1&&1\\
&&&-1&&1\\
&&&&&&1\\
&&&1&&&&1\\
&&&&&&-1&&1\\
&&&&&1&&&&1\\
&&&&&&&&&&1\\
&&&&&&&&&&-1&1
\end{bmatrix}\]
For monodromy around $z=0$
\[\begin{bmatrix}
1\\
&1\\
&&1\\
&&&1\\
&&&&1\\
&&&&&1\\
&&&&&&1\\
&&&1&&&&1\\
&&&&&&&&1\\
&&&&&&&&&1\\
&&&&&&&&&&1\\
&&&&&&&&&&&1
\end{bmatrix}\]
For monodromy around $x=1$
\[\begin{bmatrix}
1\\
&1\\
&&1\\
&&&1\\
&&&&1\\
&&&&&1\\
&&-1&1&&&1\\
&&&&&&&1\\
&&&&-1&1&&&1\\
&&&&&&&&&1\\
&&&&&&&&&&1\\
&&&&&&&&&&&1
\end{bmatrix}\]
For monodromy around $y=1$
\[\begin{bmatrix}
1\\
&1\\
&&1\\
&&&1\\
&-1&1&&1\\
&&&&&1\\
&&&&&&1\\
&&&&&&&1\\
&&&&&-1&1&&1\\
&&&&&&&&&1\\
&&&&&&&&&&1\\
&&&&&&&&&-1&1&1
\end{bmatrix}\]
For monodromy around $z=1$
\[\begin{bmatrix}
1\\
-1&1\\
&&1\\
&&&1\\
&&-1&&1\\
&&&-1&&1\\
&&&&&&1\\
&&&&&&&1\\
&&&&&&-1&&1\\
&&&&&&&-1&&1\\
&&&&&&&&&&1\\
&&&&&&&&&&-1&1
\end{bmatrix}\]
For monodromy around $xy=1$
\[\begin{bmatrix}
1\\
&1\\
&&1\\
&&&1\\
&-1&&&1\\
&&&1&&1\\
&&&&&&1\\
&&&&&&&1\\
&&&&&&&&1\\
&&&&&&&&&1\\
&&&&&&&&&&1\\
&&&&&&&&&&&1
\end{bmatrix}\]
For monodromy around $yz=1$
\[\begin{bmatrix}
1\\
&1\\
-1&&1\\
&&&1\\
&&&&1\\
&&&&&1\\
&&&&&&1\\
&&&&&&&1\\
&&&&&&&&1\\
&&&&&&&&&1\\
&&&&&&&-1&&&1\\
&&&&&&&&&&&1
\end{bmatrix}\]
For monodromy around $xyz=1$
\[\begin{bmatrix}
1\\
&1\\
&&1\\
-1&&&1\\
&&&&1\\
&&&&&1\\
&&&&&&1\\
&&&&&&&1\\
&&&&&&&&1\\
&&&&&&&&&1\\
&&&&&&&&&&1\\
&&&&&&&&&&&1
\end{bmatrix}\]

$d\omega_{2,1,1}(x,y,z)+(\omega_2(xyz)-w_2(x))\wedge\omega_{1,1}(y,z)+(\omega_2(x)+\omega_2(y))\wedge\omega_{1,1}(xy,z)=0$, we have $d\bm{\omega}-\bm{\omega}\wedge\bm{\omega}=0$ for
\[\bm{\omega}=\begin{bmatrix}
0\\
\omega_{1,1}(y,z)&0\\
\omega_{1,1}(xy,z)&0&0\\
\omega_{2}(xyz)&0&0&0\\
\omega_{2,1,1}(x,y,z)&\omega_2(x)&-\omega_2(x)-\omega_2(y)&\omega_{1,1}(y,z)&0
\end{bmatrix}\]

And the variation matrix should be
\[
\begin{bmatrix}
1\\
\widehat{\mathcal L}_{1,1}(y,z)&1\\
\widehat{\mathcal L}_{1,1}(xy,z)&0&1\\
\widehat{\mathcal L}_{2}(xyz)&0&0&1\\
\widehat{\mathcal L}_{2,1,1}(x,y,z)&\widehat{\mathcal L}_2(x)&-\widehat{\mathcal L}_2(x)-\widehat{\mathcal L}_2(y)&\widehat{\mathcal L}_{1,1}(y,z)&1\\
\end{bmatrix}
\]

Here
\[\widehat{\mathcal L}_{1,1}(x,y)=\Li_{1,1}(x,y)-\frac{1}{2}(v_{12} v_2-v_1 v_2 + v_1 v_{12} - u_1 v_{12})\]
\[\widehat{\mathcal L}_{2}(x)=\Li_{2}(x)+\frac{1}{2}v_1u_1\]
\begin{align*}
\widehat{\mathcal L}_{2,1,1}(x,y,z)&=\Li_{2,1,1}(x,y,z) + (v_3 - v_2 + u_2) \Li_{2, 1}(x,yz) + v_2 \Li_{2, 1}(xy,z) - u_1 \Li_{1, 1, 1}(x,y,z) \\
&+  \frac{1}{2} (v_{23} (v_3 + u_2 - v_2) + v_2 v_3) \Li_{2}(xyz) - (u_1 (v_3 + u_2 - v_2)) \Li_{1, 1}(x,yz)\\
&+ \left(-u_1 v_2 - \frac{1}{2} u_1^2 +\frac{1}{2} u_1 v_1 - \frac{1}{2} u_2 v_2\right) \Li_{1,1}(xy,z) - \frac{1}{2} u_1 v_1\Li_{1, 1}(y,z)
\end{align*}

The unipotent monodromy representation would be
$x=0,xyz=1$
\[
\begin{bmatrix}
1\\
&1\\
1&&1\\
-1&&&1\\
-\frac{7}{12}&&&&1
\end{bmatrix}
\]
$y=0,xyz=1$
\[
\begin{bmatrix}
1\\
&1\\
1&&1\\
-1&&&1\\
-\frac{1}{12}&&&&1
\end{bmatrix}
\]
$y=0,yz=1$
\[
\begin{bmatrix}
1\\
1&1\\
&&1\\
&&&1\\
&&&1&1
\end{bmatrix}
\]
$z=0,xyz=1$
\[
\begin{bmatrix}
1\\
&1\\
&&1\\
-1&&&1\\
&&&&1
\end{bmatrix}
\]
$xy=1,xyz=1$
\[
\begin{bmatrix}
1\\
&1\\
-1&&1\\
&&&1\\
\frac{1}{12}&&&&1
\end{bmatrix}
\]
$xy=1,z=1$
\[
\begin{bmatrix}
1\\
&1\\
1&&1\\
&&&1\\
-\frac{1}{12}&&&&1
\end{bmatrix}
\]
$xyz=1,z=1$
\[
\begin{bmatrix}
1\\
&1\\
-1&&1\\
&&&1\\
\frac{1}{12}&&&&1
\end{bmatrix}
\]
$y=1,yz=1$
\[
\begin{bmatrix}
1\\
-1&1\\
&&1\\
&&&1\\
&&&&1
\end{bmatrix}
\]
$y=1,z=1$
\[
\begin{bmatrix}
1\\
1&1\\
&&1\\
&&&1\\
&&&&1
\end{bmatrix}
\]
$yz=1,z=1$
\[
\begin{bmatrix}
1\\
-1&1\\
&&1\\
&&&1\\
&&&&1
\end{bmatrix}
\]

\end{document}